Spikes/Spike2Fibonacci/Windows/RowIndexTwoDivision.lean
@@ -1,5 +1,18 @@
-/- Copyright 2026 Craig Tiller -/
-import Spikes.Spike2Fibonacci.Windows.RowIndexTwoBranch
+/-
+Copyright 2026 Craig Tiller
+
+Licensed under the Apache License, Version 2.0 (the "License");
+you may not use this file except in compliance with the License.
+You may obtain a copy of the License at
+
+    http://www.apache.org/licenses/LICENSE-2.0
+
+Unless required by applicable law or agreed to in writing, software
+distributed under the License is distributed on an "AS IS" BASIS,
+WITHOUT WARRANTIES OR CONDITIONS OF ANY KIND, either express or implied.
+See the License for the specific language governing permissions and
+limitations under the License.
+-/import Spikes.Spike2Fibonacci.Windows.RowIndexTwoBranch
 
 namespace Spikes.Spike2Fibonacci.Windows
 
@@ -37,6 +50,7 @@ opaque spike2_two_digit_division_slice (state : X86_64MachineState)
     final := final
     certificate := spike2_two_digit_division_selected_prefix state eventsRev hrip safe
     registers := frame
+    fibRegisters := spike2_two_digit_division_fibRegisterFrame state
     rip := finalRip
     rsp := frame.rsp.trans rsp
     fault := frame.fault.trans safe
